Snapshot, with one puzzling assume in Views.fst and a broken proof in HMAC :'(

vale/code/arch/x64/Views.fst
@@ -85,3 +85,44 @@ let inverses128 (u:unit) =
   in
   Classical.forall_intro aux1;
   Classical.forall_intro aux2
+
+let get32_128_aux1 (x: Seq.lseq U32.t 4): Lemma (put32_128 (get32_128 x) == x) =
+  reveal_opaque put32_128_def;
+  reveal_opaque get32_128_def;
+  let vg = get32_128 x in
+  let vp = put32_128 vg in
+  assert (Seq.index vp 0 = UInt32.uint_to_t vg.lo0);
+  assert (Seq.index vp 1 = UInt32.uint_to_t vg.lo1);
+  assert (Seq.index vp 2 = UInt32.uint_to_t vg.hi2);
+  assert (Seq.index vp 3 = UInt32.uint_to_t vg.hi3);
+  assert (Seq.equal x vp)
+
+let put32_128_aux1 (x: quad32): Lemma (get32_128 (put32_128 x) == x) =
+  reveal_opaque put32_128_def;
+  reveal_opaque get32_128_def;
+  let vp = put32_128 x in
+  let vg = get32_128 vp in
+  assert (vg == Mkfour
+    (U32.v (Seq.index vp 0))
+    (U32.v (Seq.index vp 1))
+    (U32.v (Seq.index vp 2))
+    (U32.v (Seq.index vp 3)));
+  assert (Seq.index vp 0 == UInt32.uint_to_t x.lo0);
+  assert (Seq.index vp 1 == UInt32.uint_to_t x.lo1);
+  assert (Seq.index vp 2 == UInt32.uint_to_t x.hi2);
+  assert (Seq.index vp 3 == UInt32.uint_to_t x.hi3);
+  assert (vg == Mkfour
+    (U32.v (UInt32.uint_to_t x.lo0))
+    (U32.v (UInt32.uint_to_t x.lo1))
+    (U32.v (UInt32.uint_to_t x.hi2))
+    (U32.v (UInt32.uint_to_t x.hi3)));
+  assert (vg == Mkfour x.lo0 x.lo1 x.hi2 x.hi3);
+  assert (Mkfour x.lo0 x.lo1 x.hi2 x.hi3 == x);
+  assume (vg == x)
+
+let inverses32_128 (u:unit) =
+  reveal_opaque get32_128_def;
+  reveal_opaque put32_128_def;
+  Classical.forall_intro get32_128_aux1;
+  Classical.forall_intro put32_128_aux1
+
